Clean this up by adding comments and doing a little re-ordering.

examples/lambda/pure_dBScript.sml
@@ -1,11 +1,16 @@
 open HolKernel boolLib Parse bossLib pred_setTheory termTheory BasicProvers
 
+open arithmeticTheory boolSimps
+
 local open string_numTheory in end
 
 val _ = new_theory "pure_dB"
 
+(* the type of pure de Bruijn terms *)
 val _ = Hol_datatype`pdb = dV of num | dAPP of pdb => pdb | dABS of pdb`
 
+(* Definitions of lift and substitution from Nipkow's "More Church-Rosser
+   proofs" *)
 val lift_def = Define`
   (lift (dV i) k = if i < k then dV i else dV (i + 1)) /\
   (lift (dAPP s t) k = dAPP (lift s k) (lift t k)) /\
@@ -13,25 +18,30 @@ val lift_def = Define`
 `;
 val _ = export_rewrites ["lift_def"]
 
-val dsubst_def = Define`
-  (dsubst s k (dV i) = if k < i then dV (i - 1)
+(* "Nipkow" substitution *)
+val nsub_def = Define`
+  (nsub s k (dV i) = if k < i then dV (i - 1)
                        else if i = k then s else dV i) /\
-  (dsubst s k (dAPP t u) = dAPP (dsubst s k t) (dsubst s k u)) /\
-  (dsubst s k (dABS t) = dABS (dsubst (lift s 0) (k + 1) t))
+  (nsub s k (dAPP t u) = dAPP (nsub s k t) (nsub s k u)) /\
+  (nsub s k (dABS t) = dABS (nsub (lift s 0) (k + 1) t))
 `;
-val _ = export_rewrites ["dsubst_def"]
+val _ = export_rewrites ["nsub_def"]
 
-val pdsubst_def = Define`
-  (pdsubst s k (dV i) = if i = k then s else dV i) /\
-  (pdsubst s k (dAPP t u) = dAPP (pdsubst s k t) (pdsubst s k u)) /\
-  (pdsubst s k (dABS t) = dABS (pdsubst (lift s 0) (k + 1) t))
+(* substitution that corresponds to substitution in the lambda-calculus;
+   no variable decrementing in the dV clause *)
+val sub_def = Define`
+  (sub s k (dV i) = if i = k then s else dV i) /\
+  (sub s k (dAPP t u) = dAPP (sub s k t) (sub s k u)) /\
+  (sub s k (dABS t) = dABS (sub (lift s 0) (k + 1) t))
 `;
-val _ = export_rewrites ["pdsubst_def"]
+val _ = export_rewrites ["sub_def"]
 
+(* a variable-binding lambda-equivalent for dB terms *)
 val dLAM_def = Define`
-  dLAM v body = dABS (pdsubst (dV 0) (v + 1) (lift body 0))
+  dLAM v body = dABS (sub (dV 0) (v + 1) (lift body 0))
 `
 
+(* the set of free indices in a term *)
 val dFV_def = Define`
   (dFV (dV i) = {i}) /\
   (dFV (dAPP t u) = dFV t UNION dFV u) /\
@@ -45,8 +55,11 @@ val FINITE_dFV = store_thm(
   Induct_on `t` THEN SRW_TAC [][]);
 val _ = export_rewrites ["FINITE_dFV"]
 
+(* guarded increment of a string: it's untouched if the corresponding index
+   is less than the guard, otherwise it's bumped, and then pushed back into
+   the string type *)
 val ginc_def = Define`
-  ginc gd i = if s2n i < gd then i else n2s (s2n i + 1)
+  ginc gd s = if s2n s < gd then s else n2s (s2n s + 1)
 `
 
 val ginc_0 = store_thm(
@@ -79,6 +92,8 @@ val ginc_neq = store_thm(
   ]);
 val _ = export_rewrites ["ginc_neq"]
 
+(* incrementing a permutation, defined in terms of the underlying list of
+   pairs representation *)
 val inc_pm_def = Define`
   (inc_pm g [] = []) /\
   (inc_pm g ((x,y)::rest) = (ginc g x, ginc g y) :: inc_pm g rest)
@@ -90,6 +105,7 @@ val inc_pm_APPEND = store_thm(
   ``!pi1 pi2. inc_pm g (pi1 ++ pi2) = inc_pm g pi1 ++ inc_pm g pi2``,
   Induct THEN ASM_SIMP_TAC (srw_ss()) [pairTheory.FORALL_PROD]);
 
+(* characterisation of what an incremented permutation does to a string *)
 val lswapstr_inc_pm = store_thm(
   "lswapstr_inc_pm",
   ``!pi g s. lswapstr (inc_pm g pi) s =
@@ -109,6 +125,7 @@ val inc_pm_permeq = store_thm(
   SIMP_TAC (srw_ss()) [nomsetTheory.permeq_def, lswapstr_inc_pm,
                        FUN_EQ_THM]);
 
+(* definition of permutation over de Bruijn terms *)
 val dpm_def = Define`
   (dpm pi (dV i) = dV (s2n (lswapstr pi (n2s i)))) /\
   (dpm pi (dAPP t u) = dAPP (dpm pi t) (dpm pi u)) /\
@@ -116,6 +133,7 @@ val dpm_def = Define`
 `;
 val _ = export_rewrites ["dpm_def"]
 
+(* proof that dB terms + dpm form a nominal set *)
 val dpm_is_perm = store_thm(
   "dpm_is_perm",
   ``is_perm dpm``,
@@ -129,6 +147,19 @@ val dpm_is_perm = store_thm(
   ]);
 val _ = export_rewrites ["dpm_is_perm"]
 
+(* being a nominal set gives us properties of dpm "for free" *)
+val dpm_flip_args = store_thm(
+  "dpm_flip_args",
+  ``dpm ((x,y)::pi) t = dpm ((y,x)::pi) t``,
+  SRW_TAC [][nomsetTheory.is_perm_flip_args]);
+
+val dpm_sing_inv = store_thm(
+  "dpm_sing_inv",
+  ``dpm [h] (dpm [h] t) = t``,
+  SRW_TAC [][nomsetTheory.is_perm_sing_inv]);
+val _ = export_rewrites ["dpm_sing_inv"]
+
+(* dFVs gives the free indices of a dB term as strings *)
 val dFVs_def = Define`dFVs t = IMAGE n2s (dFV t)`
 val dFVs_thm = store_thm(
   "dFVs_thm",
@@ -150,6 +181,8 @@ val FINITE_dFVs = store_thm(
   SRW_TAC [][dFVs_def]);
 val _ = export_rewrites ["FINITE_dFVs"]
 
+(* this and the next result establish that dFVs gives the support of a
+   dB term *)
 val dpm_apart = store_thm(
   "dpm_apart",
   ``!x y. x IN dFVs t /\ ~(y IN dFVs t) ==> ~(dpm [(x,y)] t = t)``,
@@ -186,11 +219,29 @@ val dpm_supp = store_thm(
   MATCH_MP_TAC dpm_fresh THEN SRW_TAC [][]);
 val _ = export_rewrites ["dpm_supp"]
 
-val dpm_sing_inv = store_thm(
-  "dpm_sing_inv",
-  ``dpm [h] (dpm [h] t) = t``,
-  SRW_TAC [][nomsetTheory.is_perm_sing_inv]);
-val _ = export_rewrites ["dpm_sing_inv"]
+
+(* this is enough to establish de Bruijn terms as a nominal type for the
+   purposes of function definition.  I.e., now we can define functions
+   that have dB terms as their range *)
+val _ = binderLib.range_database :=
+        Binarymap.insert(!binderLib.range_database, "pdb",
+                         {nullfv = ``dABS (dV 0)``,
+                          rewrites = [],
+                          inst = ["rFV" |-> (fn () => ``pure_dB$dFVs``),
+                                  "rswap" |-> (fn () =>
+                                                  ``\x y t. dpm [(x,y)] t``),
+                                  "apm" |-> (fn () => ``pure_dB$dpm``)]})
+
+
+
+(* substitution of a fresh variable is actually a permutation *)
+val fresh_dpm_sub = prove(
+  ``!i j M. ~(j IN dFV M) ==> (sub (dV j) i M = dpm [(n2s j, n2s i)] M)``,
+  Induct_on `M` THEN SRW_TAC [][ginc_0] THEN
+  FIRST_X_ASSUM MATCH_MP_TAC THEN
+  FIRST_X_ASSUM (Q.SPEC_THEN `j + 1` MP_TAC) THEN SRW_TAC [][PRE_SUB1]);
+
+
 
 val ginc_0n = prove(
   ``ginc 0 (ginc n s) = ginc (n + 1) (ginc 0 s)``,
@@ -200,6 +251,7 @@ val inc_pm_0n = prove(
   ``!pi. inc_pm 0 (inc_pm n pi) = inc_pm (n + 1) (inc_pm 0 pi)``,
   Induct THEN ASM_SIMP_TAC (srw_ss()) [pairTheory.FORALL_PROD, ginc_0n])
 
+(* interaction of lifting and permutation *)
 val lift_dpm = store_thm(
   "lift_dpm",
   ``!n pi. lift (dpm pi M) n = dpm (inc_pm n pi) (lift M n)``,
@@ -212,62 +264,60 @@ val lift_dpm = store_thm(
     SRW_TAC [][inc_pm_0n]
   ]);
 
-val dpm_pdsubst = store_thm(
-  "dpm_pdsubst",
+(* substitution and permutation are clean *)
+val dpm_sub = store_thm(
+  "dpm_sub",
   ``!pi M j N.
-        dpm pi (pdsubst M j N) = pdsubst (dpm pi M) (s2n (lswapstr pi (n2s j)))
+        dpm pi (sub M j N) = sub (dpm pi M) (s2n (lswapstr pi (n2s j)))
                                          (dpm pi N)``,
   Induct_on `N` THEN SRW_TAC [][lswapstr_inc_pm, lift_dpm] THEN
   SRW_TAC [][ginc_0]);
 
+(* thus, so too is dLAM *)
 val dpm_dLAM = store_thm(
   "dpm_dLAM",
   ``dpm pi (dLAM j t) = dLAM (s2n (lswapstr pi (n2s j))) (dpm pi t)``,
-  SRW_TAC [][dLAM_def, dpm_pdsubst, lift_dpm, lswapstr_inc_pm] THEN
+  SRW_TAC [][dLAM_def, dpm_sub, lift_dpm, lswapstr_inc_pm] THEN
   SRW_TAC [][ginc_0])
 val _ = export_rewrites ["dpm_dLAM"]
 
-val pdsubst_14a = store_thm(
-  "pdsubst_14a",
-  ``!i t. pdsubst (dV i) i t = t``,
+(* some standard results about substitution *)
+val sub_14a = store_thm(
+  "sub_14a",
+  ``!i t. sub (dV i) i t = t``,
   Induct_on `t` THEN SRW_TAC [][]);
 
-val pdsubst_14b = store_thm(
-  "pdsubst_14b",
-  ``!M i N. ~(i IN dFV N) ==> (pdsubst M i N = N)``,
+val sub_14b = store_thm(
+  "sub_14b",
+  ``!M i N. ~(i IN dFV N) ==> (sub M i N = N)``,
   Induct_on `N` THEN SRW_TAC [][] THEN
   FIRST_X_ASSUM (Q.SPEC_THEN `i + 1` MP_TAC) THEN
   SRW_TAC [ARITH_ss][])
 
-val pdsubst_15a = store_thm(
-  "pdsubst_15a",
+val sub_15a = store_thm(
+  "sub_15a",
   ``!M i j N. ~(i IN dFV M) ==>
-              (pdsubst N i (pdsubst (dV i) j M) = pdsubst N j M)``,
+              (sub N i (sub (dV i) j M) = sub N j M)``,
   Induct_on `M` THEN SRW_TAC [][] THEN
   FIRST_X_ASSUM MATCH_MP_TAC THEN
   FIRST_X_ASSUM (Q.SPEC_THEN `i + 1` MP_TAC) THEN SRW_TAC [ARITH_ss][]);
 
 open chap2Theory
 
+(* from Nipkow *)
 val tn_lift_lemma1 = prove(
   ``!t i k. i < k ==> (lift (lift t i) k = lift (lift t (k - 1)) i)``,
   Induct THEN SRW_TAC [ARITH_ss][])
 
-
-val lift_pdsubst = store_thm(
-  "lift_pdsubst",
+(* result needed to establish the substitution lemma *)
+val lift_sub = store_thm(
+  "lift_sub",
   ``!M i N n.
        n <= i ==>
-       (lift (pdsubst M i N) n = pdsubst (lift M n) (i + 1) (lift N n))``,
+       (lift (sub M i N) n = sub (lift M n) (i + 1) (lift N n))``,
   Induct_on `N` THEN
   SRW_TAC [ARITH_ss][tn_lift_lemma1])
 
-
-
-
-
-
-open arithmeticTheory boolSimps
 val sn_iso_num = prove(
   ``((s = n2s n) = (n = s2n s)) /\ ((n2s n = s) = (n = s2n s))``,
   METIS_TAC [string_numTheory.s2n_n2s, string_numTheory.n2s_s2n])
@@ -301,23 +351,26 @@ val dFV_lift = store_thm(
     ]
   ]);
 
-val pdsubst_lemma = store_thm(
-  "dsubst_lemma",
+(* The substitution lemma, in dB guise *)
+val sub_lemma = store_thm(
+  "nsub_lemma",
   ``!M N i j L. ~(i = j) /\ ~(j IN dFV M) ==>
-                (pdsubst M i (pdsubst N j L) =
-                 pdsubst (pdsubst M i N) j (pdsubst M i L))``,
+                (sub M i (sub N j L) =
+                 sub (sub M i N) j (sub M i L))``,
   Induct_on `L` THEN
-  SRW_TAC [][pdsubst_14b, lift_pdsubst] THEN
+  SRW_TAC [][sub_14b, lift_sub] THEN
   FIRST_X_ASSUM MATCH_MP_TAC THEN
   SRW_TAC [][dFV_lift]);
 
-val pdsubst_dLAM = store_thm(
-  "pdsubst_dLAM",
+(* which allows us to prove that substitution interacts with dLAM in the way
+   we'd expect *)
+val sub_dLAM = store_thm(
+  "sub_dLAM",
   ``~(i IN dFV N) /\ ~(i = j) ==>
-    (pdsubst N j (dLAM i M) = dLAM i (pdsubst N j M))``,
+    (sub N j (dLAM i M) = dLAM i (sub N j M))``,
   SRW_TAC [][dLAM_def] THEN
-  SRW_TAC [][Once pdsubst_lemma, dFV_lift] THEN
-  SRW_TAC [][lift_pdsubst]);
+  SRW_TAC [][Once sub_lemma, dFV_lift] THEN
+  SRW_TAC [][lift_sub]);
 
 val dFVs_lift = store_thm(
   "dFVs_lift",
@@ -326,24 +379,25 @@ val dFVs_lift = store_thm(
   SRW_TAC [][dFVs_def, dFV_lift, EXTENSION, EQ_IMP_THM] THEN
   SRW_TAC [][]);
 
-val dFVs_pdsubst = store_thm(
-  "dFVs_pdsubst",
-  ``!M j. dFVs (pdsubst M j N) = if j IN dFV N then
+(* free variables of a substitution *)
+val dFVs_sub = store_thm(
+  "dFVs_sub",
+  ``!M j. dFVs (sub M j N) = if j IN dFV N then
                                    (dFVs N DELETE n2s j) UNION dFVs M
                                  else dFVs N``,
   SIMP_TAC (srw_ss() ++ boolSimps.COND_elim_ss) [] THEN
   SIMP_TAC (srw_ss()) [tautLib.TAUT_PROVE ``p \/ q = ~p ==> q``,
-                       FORALL_AND_THM, pdsubst_14b] THEN
+                       FORALL_AND_THM, sub_14b] THEN
   Induct_on `N` THEN SRW_TAC [][] THEN
   FULL_SIMP_TAC (srw_ss()) [] THENL [
     Cases_on `j IN dFV N'` THEN
-    SRW_TAC [][pdsubst_14b] THEN
+    SRW_TAC [][sub_14b] THEN
     SRW_TAC [][EXTENSION, EQ_IMP_THM] THEN SRW_TAC [][] THEN
     Cases_on `x = n2s j` THEN SRW_TAC [][] THEN
     FULL_SIMP_TAC (srw_ss()) [dFVs_def],
 
     Cases_on `j IN dFV N` THEN
-    SRW_TAC [][pdsubst_14b] THEN
+    SRW_TAC [][sub_14b] THEN
     SRW_TAC [][EXTENSION, EQ_IMP_THM] THEN SRW_TAC [][] THEN
     Cases_on `x = n2s j` THEN SRW_TAC [][] THEN
     FULL_SIMP_TAC (srw_ss()) [dFVs_def],
@@ -375,31 +429,18 @@ val dFVs_pdsubst = store_thm(
     ]
   ]);
 
+(* and thus, the free variables of dLAM *)
 val dFVs_dLAM = store_thm(
   "dFVs_dLAM",
   ``dFVs (dLAM i bod) = dFVs bod DELETE (n2s i)``,
-  SRW_TAC [][dLAM_def, dFVs_pdsubst, dFV_lift, dFVs_lift] THEN
+  SRW_TAC [][dLAM_def, dFVs_sub, dFV_lift, dFVs_lift] THEN
   SRW_TAC [DNF_ss][EXTENSION] THEN
   SRW_TAC [][sn_iso_num, dFVs_def] THEN
   METIS_TAC []);
 val _ = export_rewrites ["dFVs_dLAM"]
 
-val _ = binderLib.range_database :=
-        Binarymap.insert(!binderLib.range_database, "pdb",
-                         {nullfv = ``dABS (dV 0)``,
-                          rewrites = [],
-                          inst = ["rFV" |-> (fn () => ``pure_dB$dFVs``),
-                                  "rswap" |-> (fn () =>
-                                                  ``\x y t. dpm [(x,y)] t``),
-                                  "apm" |-> (fn () => ``pure_dB$dpm``)]})
-
-val (dbeta_rules, dbeta_ind, dbeta_cases) = Hol_reln`
-  (!s t. dbeta (dAPP (dABS s) t) (dsubst t 0 s)) /\
-  (!s t u. dbeta s t ==> dbeta (dAPP s u) (dAPP t u)) /\
-  (!s t u. dbeta s t ==> dbeta (dAPP u s) (dAPP u t)) /\
-  (!s t. dbeta s t ==> dbeta (dABS s) (dABS t))
-`;
-
+(* now that we know what the free variables of dLAM are, the definition
+   below can go through *)
 val (fromTerm_def,fromTerm_tpm) = binderLib.define_recursive_term_function`
   (fromTerm (VAR s) = dV (s2n s)) /\
   (fromTerm (t @@ u) = dAPP (fromTerm t) (fromTerm u)) /\
@@ -417,6 +458,10 @@ val fromTerm_eq0 = prove(
   Q.SPEC_THEN `t` STRUCT_CASES_TAC term_CASES THEN
   SRW_TAC [][fromTerm_def, dLAM_def, sn_iso_num] THEN METIS_TAC []);
 
+(* Can now show that the appropriate functions in dB and term really do
+   match up *)
+
+(* free variables *)
 val dFVs_fromTerm = store_thm(
   "dFVs_fromTerm",
   ``!N. dFVs (fromTerm N) = FV N``,
@@ -428,17 +473,13 @@ val IN_dFV = store_thm(
   ``x IN dFV t = n2s x IN dFVs t``,
   SRW_TAC [][dFVs_def]);
 
+(* substitution *)
 val fromTerm_subst = store_thm(
   "fromTerm_subst",
-  ``!M. fromTerm ([N/v] M) = pdsubst (fromTerm N) (s2n v) (fromTerm M)``,
+  ``!M. fromTerm ([N/v] M) = sub (fromTerm N) (s2n v) (fromTerm M)``,
   HO_MATCH_MP_TAC nc_INDUCTION2 THEN Q.EXISTS_TAC `v INSERT FV N` THEN
-  SRW_TAC [][SUB_THM, SUB_VAR, fromTerm_def, pdsubst_dLAM, IN_dFV]);
+  SRW_TAC [][SUB_THM, SUB_VAR, fromTerm_def, sub_dLAM, IN_dFV]);
 
-val fresh_dpm_pdsubst = prove(
-  ``!i j M. ~(j IN dFV M) ==> (pdsubst (dV j) i M = dpm [(n2s j, n2s i)] M)``,
-  Induct_on `M` THEN SRW_TAC [][ginc_0] THEN
-  FIRST_X_ASSUM MATCH_MP_TAC THEN
-  FIRST_X_ASSUM (Q.SPEC_THEN `j + 1` MP_TAC) THEN SRW_TAC [][PRE_SUB1]);
 
 val lift_11 = store_thm(
   "lift_11",
@@ -446,35 +487,30 @@ val lift_11 = store_thm(
   Induct_on `M1` THEN SRW_TAC [][] THEN Cases_on `M2` THEN
   SRW_TAC [][] THEN DECIDE_TAC);
 
-val dpm_flip_args = store_thm(
-  "dpm_flip_args",
-  ``dpm ((x,y)::pi) t = dpm ((y,x)::pi) t``,
-  SRW_TAC [][nomsetTheory.is_perm_flip_args]);
-
 val fromTerm_eqlam = prove(
   ``(fromTerm t = dLAM i d) = ?t0. (t = LAM (n2s i) t0) /\ (d = fromTerm t0)``,
   EQ_TAC THENL [
     Q.SPEC_THEN `t` STRUCT_CASES_TAC term_CASES THEN
     SRW_TAC [][fromTerm_def, dLAM_def] THEN
     Cases_on `i = s2n v` THENL [
-      FULL_SIMP_TAC (srw_ss()) [LAM_eq_thm, fresh_dpm_pdsubst, dFV_lift,
+      FULL_SIMP_TAC (srw_ss()) [LAM_eq_thm, fresh_dpm_sub, dFV_lift,
                                nomsetTheory.is_perm_injective, lift_11],
       `~(i IN dFV (fromTerm t0)) /\ ~(s2n v IN dFV d)`
          by (FIRST_X_ASSUM (MP_TAC o AP_TERM ``dFV``) THEN
              REWRITE_TAC [EXTENSION] THEN
              DISCH_THEN (fn th => Q.SPEC_THEN `i + 1` MP_TAC th THEN
                                   Q.SPEC_THEN `s2n v + 1` MP_TAC th) THEN
-             SRW_TAC [][IN_dFV, dFVs_pdsubst, dFVs_lift]) THEN
+             SRW_TAC [][IN_dFV, dFVs_sub, dFVs_lift]) THEN
       FIRST_X_ASSUM (MP_TAC o AP_TERM ``dpm [(n2s 0, n2s (i + 1))]``) THEN
-      ASM_SIMP_TAC (srw_ss()) [fresh_dpm_pdsubst, dFV_lift] THEN
-      ASM_SIMP_TAC (srw_ss()) [GSYM fresh_dpm_pdsubst, dFV_lift] THEN
+      ASM_SIMP_TAC (srw_ss()) [fresh_dpm_sub, dFV_lift] THEN
+      ASM_SIMP_TAC (srw_ss()) [GSYM fresh_dpm_sub, dFV_lift] THEN
       ONCE_REWRITE_TAC [dpm_flip_args] THEN
-      `~(i + 1 IN dFV (pdsubst (dV 0) (s2n v + 1) (lift (fromTerm t0) 0)))`
-         by (SRW_TAC [][dFVs_pdsubst, IN_dFV] THEN
+      `~(i + 1 IN dFV (sub (dV 0) (s2n v + 1) (lift (fromTerm t0) 0)))`
+         by (SRW_TAC [][dFVs_sub, IN_dFV] THEN
              SRW_TAC [][dFVs_def, dFV_lift]) THEN
-      ASM_SIMP_TAC (srw_ss())[GSYM fresh_dpm_pdsubst] THEN
-      ASM_SIMP_TAC (srw_ss()) [pdsubst_15a, dFV_lift] THEN
-      ASM_SIMP_TAC (srw_ss()) [fresh_dpm_pdsubst, dFV_lift] THEN
+      ASM_SIMP_TAC (srw_ss())[GSYM fresh_dpm_sub] THEN
+      ASM_SIMP_TAC (srw_ss()) [sub_15a, dFV_lift] THEN
+      ASM_SIMP_TAC (srw_ss()) [fresh_dpm_sub, dFV_lift] THEN
       `[(n2s (i + 1), n2s (s2n v + 1))] = inc_pm 0 [(n2s i, v)]`
          by SRW_TAC [][inc_pm_def, ginc_0] THEN
       ASM_SIMP_TAC bool_ss [GSYM lift_dpm, lift_11] THEN
@@ -490,6 +526,7 @@ val fromTerm_eqn = save_thm(
   "fromTerm_eqn",
   CONJ fromTerm_eq0 fromTerm_eqlam)
 
+(* fromTerm is injective *)
 val fromTerm_11 = store_thm(
   "fromTerm_11",
   ``!t1 t2. (fromTerm t1 = fromTerm t2) = (t1 = t2)``,
@@ -501,7 +538,7 @@ val fromTerm_11 = store_thm(
 
 val onto_lemma = prove(
   ``!t i n. ~(i IN dFV t) ==>
-            ?t0. t = pdsubst (dV n) i (lift t0 n)``,
+            ?t0. t = sub (dV n) i (lift t0 n)``,
   Induct_on `t` THEN SRW_TAC [][] THENL [
     Cases_on `n = n'` THENL [
       Cases_on `i < n'` THENL [
@@ -513,8 +550,8 @@ val onto_lemma = prove(
         Q.EXISTS_TAC `dV (n - 1)` THEN SRW_TAC [ARITH_ss][]
       ]
     ],
-    `?t0 t0'. (t = pdsubst (dV n) i (lift t0 n)) /\
-              (t' = pdsubst (dV n) i (lift t0' n))`
+    `?t0 t0'. (t = sub (dV n) i (lift t0 n)) /\
+              (t' = sub (dV n) i (lift t0' n))`
        by METIS_TAC [] THEN
     Q.EXISTS_TAC `dAPP t0 t0'` THEN SRW_TAC [][],
 
@@ -542,7 +579,7 @@ val dfresh_exists = store_thm(
   Q.EXISTS_TAC `j` THEN STRIP_TAC THEN RES_TAC THEN
   FULL_SIMP_TAC (srw_ss()) []);
 
-
+(* a cases theorem for dB based around dLAM rather than dSUB *)
 val db_cases' = store_thm(
   "db_cases'",
   ``!t. (?i. t = dV i) \/ (?t0 t1. t = dAPP t0 t1) \/
@@ -553,55 +590,41 @@ val db_cases' = store_thm(
      by (STRIP_TAC THEN RES_TAC THEN DECIDE_TAC) THEN
   METIS_TAC [onto_lemma]);
 
-val dbsize_def = Define`
-  (dbsize (dV i) = 1) /\
-  (dbsize (dAPP d1 d2) = dbsize d1 + dbsize d2 + 1) /\
-  (dbsize (dABS d) = dbsize d + 1)
-`
-val _ = export_rewrites ["dbsize_def"]
-
-val dbsize_pdsubst = store_thm(
-  "dbsize_pdsubst",
-  ``!n i M. dbsize (pdsubst (dV n) i M) = dbsize M``,
-  Induct_on `M` THEN SRW_TAC [][]);
-val _ = export_rewrites ["dbsize_pdsubst"]
-
-val dbsize_lift = store_thm(
-  "dbsize_lift",
-  ``!n M. dbsize (lift M n) = dbsize M``,
-  Induct_on `M` THEN SRW_TAC [][]);
-val _ = export_rewrites ["dbsize_lift"]
-
-val dbsize_dLAM = store_thm(
-  "dbsize_dLAM",
-  ``dbsize (dLAM i t) = dbsize t + 1``,
-  SRW_TAC [][dLAM_def])
-val _ = export_rewrites ["dbsize_dLAM"]
-
-
-val pdsubst_dsubst = store_thm(
-  "pdsubst_dsubst",
+val sub_nsub = store_thm(
+  "sub_nsub",
   ``!N i n M.
        n <= i ==>
-       (pdsubst N i M = dsubst N n (pdsubst (dV n) (i + 1) (lift M n)))``,
+       (sub N i M = nsub N n (sub (dV n) (i + 1) (lift M n)))``,
   Induct_on `M` THEN SRW_TAC [][] THENL [
     SRW_TAC [ARITH_ss][] THEN FULL_SIMP_TAC (srw_ss() ++ ARITH_ss) [],
     SRW_TAC [ARITH_ss][],
     SRW_TAC [ARITH_ss][]
   ]);
 
+
+(* Nipkow's definition of beta reduction *)
+val (dbeta_rules, dbeta_ind, dbeta_cases) = Hol_reln`
+  (!s t. dbeta (dAPP (dABS s) t) (nsub t 0 s)) /\
+  (!s t u. dbeta s t ==> dbeta (dAPP s u) (dAPP t u)) /\
+  (!s t u. dbeta s t ==> dbeta (dAPP u s) (dAPP u t)) /\
+  (!s t. dbeta s t ==> dbeta (dABS s) (dABS t))
+`;
+
+(* all of the "lambda-calculus" redexes reduce appropriately under dbeta *)
 val alt_dbeta_rule = store_thm(
   "alt_dbeta_rule",
-  ``dbeta (dAPP (dLAM i M) N) (pdsubst N i M)``,
+  ``dbeta (dAPP (dLAM i M) N) (sub N i M)``,
   SRW_TAC [][dLAM_def] THEN
-  Q_TAC SUFF_TAC `pdsubst N i M =
-                  dsubst N 0 (pdsubst (dV 0) (i + 1) (lift M 0))`
+  Q_TAC SUFF_TAC `sub N i M =
+                  nsub N 0 (sub (dV 0) (i + 1) (lift M 0))`
         THEN1 (DISCH_THEN SUBST1_TAC THEN
                MATCH_ACCEPT_TAC (hd (CONJUNCTS dbeta_rules))) THEN
-  MATCH_MP_TAC pdsubst_dsubst THEN SRW_TAC [][]);
+  MATCH_MP_TAC sub_nsub THEN SRW_TAC [][]);
 
+(* an alternative reduction relation that is a stepping stone between
+   dbeta and beta-reduction on quotiented terms *)
 val (dbeta'_rules, dbeta'_ind, dbeta'_cases) = Hol_reln`
-  (!i M N. dbeta' (dAPP (dLAM i M) N) (pdsubst N i M)) /\
+  (!i M N. dbeta' (dAPP (dLAM i M) N) (sub N i M)) /\
   (!M N Z. dbeta' M N ==> dbeta' (dAPP M Z) (dAPP N Z)) /\
   (!M N Z. dbeta' M N ==> dbeta' (dAPP Z M) (dAPP Z N)) /\
   (!M N i. dbeta' M N ==> dbeta' (dLAM i M) (dLAM i N))
@@ -616,28 +639,34 @@ val dABS_renamed = store_thm(
 
 val dbeta'_dpm = prove(
   ``!M N. dbeta' M N ==> !pi. dbeta' (dpm pi M) (dpm pi N)``,
-  HO_MATCH_MP_TAC dbeta'_ind THEN SRW_TAC [][dpm_pdsubst, dbeta'_rules]);
+  HO_MATCH_MP_TAC dbeta'_ind THEN SRW_TAC [][dpm_sub, dbeta'_rules]);
 
 val dbeta'_dpm_calc = store_thm(
   "dbeta'_dpm_calc",
   ``!M N. dbeta' (dpm pi M) N = dbeta' M (dpm (REVERSE pi) N)``,
   METIS_TAC [dbeta'_dpm, nomsetTheory.is_perm_inverse, dpm_is_perm])
 
-val inc_as_pm_def = Define`
-  inc_as_pm lim n = if n < lim then []
+(* We can construct a lift permutation.
+     inc_as_pm lim n
+   constructs a permutation that will bring about the effect of
+     lift M lim
+   as long as n is as big as the biggest free index in M
+*)
+val lifting_pm_def = Define`
+  lifting_pm lim n = if n < lim then []
                     else if n = lim then [(n2s n, n2s (n + 1))]
-                    else inc_as_pm lim (n - 1) ++ [(n2s n, n2s (n + 1))]
+                    else lifting_pm lim (n - 1) ++ [(n2s n, n2s (n + 1))]
 `
 
-val inc_as_pm_behaves = store_thm(
-  "inc_as_pm_behaves",
+val lifting_pm_behaves = store_thm(
+  "lifting_pm_behaves",
   ``!n lim i.
-      lswapstr (inc_as_pm lim n) (n2s i) =
+      lswapstr (lifting_pm lim n) (n2s i) =
           if i < lim then n2s i
           else if i <= n then n2s (i + 1)
           else if i = n + 1 then n2s lim
           else n2s i``,
-  Induct THEN ONCE_REWRITE_TAC [inc_as_pm_def] THENL [
+  Induct THEN ONCE_REWRITE_TAC [lifting_pm_def] THENL [
     SRW_TAC [][] THEN FULL_SIMP_TAC (srw_ss() ++ ARITH_ss) [],
     REPEAT GEN_TAC THEN Cases_on `SUC n < lim` THENL [
       ASM_SIMP_TAC (srw_ss()) [] THEN
@@ -666,10 +695,11 @@ val inc_as_pm_behaves = store_thm(
     ]
   ]);
 
-val inc_pm0_inc_as_pm = store_thm(
-  "inc_pm0_inc_as_pm",
-  ``!m n. inc_pm 0 (inc_as_pm m n) = inc_as_pm (m + 1) (n + 1)``,
-  Induct_on `n` THEN ONCE_REWRITE_TAC [inc_as_pm_def] THENL [
+(* interaction of inc_pm with lifting_pm *)
+val inc_pm0_lifting_pm = store_thm(
+  "inc_pm0_lifting_pm",
+  ``!m n. inc_pm 0 (lifting_pm m n) = lifting_pm (m + 1) (n + 1)``,
+  Induct_on `n` THEN ONCE_REWRITE_TAC [lifting_pm_def] THENL [
     SRW_TAC [][ginc_0] THEN
     FULL_SIMP_TAC (srw_ss() ++ ARITH_ss) [],
 
@@ -679,10 +709,10 @@ val inc_pm0_inc_as_pm = store_thm(
 val lifts_are_specific_dpms = store_thm(
   "lifts_are_specific_dpms",
   ``!M n. (!i. i IN dFV M ==> i <= n) ==>
-          !m. lift M m = dpm (inc_as_pm m n) M``,
+          !m. lift M m = dpm (lifting_pm m n) M``,
   Induct THEN SRW_TAC [][] THENL [
-    SRW_TAC [][inc_as_pm_behaves],
-    FULL_SIMP_TAC (srw_ss() ++ DNF_ss) [inc_pm0_inc_as_pm] THEN
+    SRW_TAC [][lifting_pm_behaves],
+    FULL_SIMP_TAC (srw_ss() ++ DNF_ss) [inc_pm0_lifting_pm] THEN
     FIRST_X_ASSUM MATCH_MP_TAC THEN SRW_TAC [][] THEN
     Cases_on `i = 0` THENL [
       SRW_TAC [][],
@@ -695,7 +725,7 @@ val lifts_are_dpms = store_thm(
   ``!M n. ?pi. lift M n = dpm pi M``,
   REPEAT GEN_TAC THEN
   Q.SPEC_THEN `M` STRIP_ASSUME_TAC onto_lemma2 THEN
-  Q.EXISTS_TAC `inc_as_pm n j` THEN MATCH_MP_TAC lifts_are_specific_dpms THEN
+  Q.EXISTS_TAC `lifting_pm n j` THEN MATCH_MP_TAC lifts_are_specific_dpms THEN
   REPEAT STRIP_TAC THEN RES_TAC THEN DECIDE_TAC);
 
 val dbeta'_lift = store_thm(
@@ -704,7 +734,7 @@ val dbeta'_lift = store_thm(
   Q.SPEC_THEN `M` STRIP_ASSUME_TAC onto_lemma2 THEN
   Q.SPEC_THEN `N` STRIP_ASSUME_TAC onto_lemma2 THEN
   Q.ABBREV_TAC `k = if j < j' then j' else j` THEN
-  `(lift M n = dpm (inc_as_pm n k) M) /\ (lift N n = dpm (inc_as_pm n k) N)`
+  `(lift M n = dpm (lifting_pm n k) M) /\ (lift N n = dpm (lifting_pm n k) N)`
      by (CONJ_TAC THEN MATCH_MP_TAC lifts_are_specific_dpms THEN
          REPEAT STRIP_TAC THEN RES_TAC THEN Q.UNABBREV_TAC `k` THEN
          DECIDE_TAC) THEN
@@ -717,7 +747,7 @@ val dbeta_dbeta' = store_thm(
     Q.SPEC_THEN `dABS s` STRIP_ASSUME_TAC db_cases' THEN
     FULL_SIMP_TAC (srw_ss()) [] THEN
     FULL_SIMP_TAC (srw_ss()) [dLAM_def] THEN
-    SRW_TAC [][GSYM pdsubst_dsubst] THEN
+    SRW_TAC [][GSYM sub_nsub] THEN
     SRW_TAC [][GSYM dLAM_def, dbeta'_rules],
 
     `?v. ~(v IN dFV (dABS s)) /\ ~(v IN dFV (dABS t))`
@@ -727,14 +757,15 @@ val dbeta_dbeta' = store_thm(
     `?s' t'. (dABS s = dLAM v s') /\ (dABS t = dLAM v t')`
        by METIS_TAC [dABS_renamed] THEN
     Q_TAC SUFF_TAC `dbeta' s' t'` THEN1 SRW_TAC [][dbeta'_rules] THEN
-    FULL_SIMP_TAC (srw_ss()) [dLAM_def, fresh_dpm_pdsubst, dFV_lift,
+    FULL_SIMP_TAC (srw_ss()) [dLAM_def, fresh_dpm_sub, dFV_lift,
                               dbeta'_dpm_calc, dbeta'_lift]
   ]);
 
-val dpm_dsubst = store_thm(
-  "dpm_dsubst",
+(* nsub must be icky - just look at how it behaves under permutations *)
+val dpm_nsub = store_thm(
+  "dpm_nsub",
   ``!M i pi.
-       dpm pi (dsubst M i N) = dsubst (dpm pi M) i (dpm (inc_pm i pi) N)``,
+       dpm pi (nsub M i N) = nsub (dpm pi M) i (dpm (inc_pm i pi) N)``,
   Induct_on `N` THENL [
     SIMP_TAC (srw_ss()) [] THEN REPEAT GEN_TAC THEN Cases_on `i < n` THENL [
       ASM_SIMP_TAC (srw_ss()) [] THEN
@@ -770,7 +801,7 @@ val dpm_dsubst = store_thm(
 val dbeta_dpm = store_thm(
   "dbeta_dpm",
   ``!M N. dbeta M N ==> !pi. dbeta (dpm pi M) (dpm pi N)``,
-  HO_MATCH_MP_TAC dbeta_ind THEN SRW_TAC [][dbeta_rules, dpm_dsubst])
+  HO_MATCH_MP_TAC dbeta_ind THEN SRW_TAC [][dbeta_rules, dpm_nsub])
 
 val dbeta_lift = store_thm(
   "dbeta_lift",
@@ -778,7 +809,7 @@ val dbeta_lift = store_thm(
   Q.SPEC_THEN `M` STRIP_ASSUME_TAC onto_lemma2 THEN
   Q.SPEC_THEN `N` STRIP_ASSUME_TAC onto_lemma2 THEN
   Q.ABBREV_TAC `k = if j < j' then j' else j` THEN
-  `(lift M n = dpm (inc_as_pm n k) M) /\ (lift N n = dpm (inc_as_pm n k) N)`
+  `(lift M n = dpm (lifting_pm n k) M) /\ (lift N n = dpm (lifting_pm n k) N)`
      by (CONJ_TAC THEN MATCH_MP_TAC lifts_are_specific_dpms THEN
          REPEAT STRIP_TAC THEN RES_TAC THEN Q.UNABBREV_TAC `k` THEN
          DECIDE_TAC) THEN
@@ -789,7 +820,7 @@ val dbeta'_dbeta = store_thm(
   ``!M N. dbeta' M N ==> dbeta M N``,
   HO_MATCH_MP_TAC dbeta'_ind THEN
   SRW_TAC [][dbeta_rules, alt_dbeta_rule] THEN
-  SRW_TAC [][dLAM_def, fresh_dpm_pdsubst, dFV_lift, dbeta_rules, dbeta_dpm,
+  SRW_TAC [][dLAM_def, fresh_dpm_sub, dFV_lift, dbeta_rules, dbeta_dpm,
              dbeta_lift])
 
 val dbeta_dbeta'_eqn = store_thm(
@@ -797,6 +828,11 @@ val dbeta_dbeta'_eqn = store_thm(
   ``dbeta = dbeta'``,
   SRW_TAC [][FUN_EQ_THM] THEN METIS_TAC [dbeta'_dbeta, dbeta_dbeta'])
 
+(* We've shown that dbeta and dbeta' are equivalent.  Now we use this to
+   show that dbeta matches up with beta on terms, and then we're all done *)
+
+(* both of the next two proofs begin by rewriting dbeta to dbeta', using
+   dbeta_dbeta'_eqn *)
 open chap3Theory
 val ccbeta_dbeta1 = prove(
   ``!M N. compat_closure beta M N ==> dbeta (fromTerm M) (fromTerm N)``,
@@ -811,7 +847,7 @@ val ccbeta_dbeta2 = prove(
   SRW_TAC [][fromTerm_eqn, compat_closure_rules] THEN
   FULL_SIMP_TAC (srw_ss()) [fromTerm_11] THEN
   SRW_TAC [][compat_closure_rules] THEN
-  `pdsubst (fromTerm t2) i (fromTerm t0) = fromTerm ([t2/n2s i] t0)`
+  `sub (fromTerm t2) i (fromTerm t0) = fromTerm ([t2/n2s i] t0)`
      by SRW_TAC [][fromTerm_subst] THEN
   FULL_SIMP_TAC (srw_ss()) [fromTerm_11] THEN
   SRW_TAC [][] THEN
@@ -822,6 +858,34 @@ val dbeta_ccbeta_eqn = store_thm(
   "dbeta_ccbeta_eqn",
   ``dbeta (fromTerm M) (fromTerm N) = compat_closure beta M N``,
   METIS_TAC [ccbeta_dbeta2, ccbeta_dbeta1]);
+
+(* to finish, a demonstration that fromTerm is also onto, using a size
+   measure on dB terms.  Could alternatively prove an induction
+   principle for dB in terms of dLAM.  *)
+val dbsize_def = Define`
+  (dbsize (dV i) = 1) /\
+  (dbsize (dAPP d1 d2) = dbsize d1 + dbsize d2 + 1) /\
+  (dbsize (dABS d) = dbsize d + 1)
+`
+val _ = export_rewrites ["dbsize_def"]
+
+val dbsize_sub = store_thm(
+  "dbsize_sub",
+  ``!n i M. dbsize (sub (dV n) i M) = dbsize M``,
+  Induct_on `M` THEN SRW_TAC [][]);
+val _ = export_rewrites ["dbsize_sub"]
+
+val dbsize_lift = store_thm(
+  "dbsize_lift",
+  ``!n M. dbsize (lift M n) = dbsize M``,
+  Induct_on `M` THEN SRW_TAC [][]);
+val _ = export_rewrites ["dbsize_lift"]
+
+val dbsize_dLAM = store_thm(
+  "dbsize_dLAM",
+  ``dbsize (dLAM i t) = dbsize t + 1``,
+  SRW_TAC [][dLAM_def])
+val _ = export_rewrites ["dbsize_dLAM"]
 
 val fromTerm_onto = store_thm(
   "fromTerm_onto",
